pcuic/theories/PCUICUnivSubstitution.v
@@ -2,123 +2,784 @@
 
 (** * Universe Substitution lemmas for typing derivations. *)
 
-From Coq Require Import Bool String List BinPos Compare_dec Arith Lia.
+From Coq Require Import Bool String List BinPos Compare_dec Arith Lia ZArith
+     CRelationClasses.
 Require Import Coq.Program.Syntax Coq.Program.Basics.
 From MetaCoq.Template Require Import utils config AstUtils UnivSubst.
 From MetaCoq.PCUIC Require Import PCUICAst PCUICAstUtils PCUICInduction
      PCUICLiftSubst PCUICEquality
      PCUICUnivSubst PCUICTyping PCUICWeakeningEnv PCUICClosed
-     PCUICReduction PCUICCumulativity PCUICWeakening PCUICUnivSubst.
-(* Require Import ssreflect. *)
+     PCUICReduction PCUICCumulativity PCUICWeakening.
 
 Local Set Keyed Unification.
 
-Lemma fix_context_subst_instance:
-  forall (mfix : list (def term)) (u : universe_instance),
-    fix_context (map (map_def (subst_instance_constr u) (subst_instance_constr u)) mfix) =
-    map (map_decl (subst_instance_constr u)) (fix_context mfix).
-Proof.
-  intros mfix u.
-Admitted.
+Module CS := ConstraintSet.
+Module LS := LevelSet.
 
-Lemma isWfArity_subst_instance:
-  forall (cf : checker_flags) (Σ : global_env × universes_decl) (Γ : context) (B : term),
-    isWfArity typing Σ Γ B ->
-    forall (u : universe_instance) (univs : universes_decl),
-      consistent_instance_ext (Σ.1, univs) Σ.2 u ->
-      isWfArity typing (Σ.1, univs) (subst_instance_context u Γ) (subst_instance_constr u B).
+Create HintDb univ_subst.
+
+Local Ltac aa := rdestruct; eauto with univ_subst.
+
+
+Section CheckerFlags.
+Context {cf : checker_flags}.
+
+
+Global Instance subst_instance_list {A} `(UnivSubst A) : UnivSubst (list A)
+  := fun u => map (subst_instance u).
+
+Global Instance subst_instance_def {A : Set} `(UnivSubst A) : UnivSubst (def A)
+  := fun u => map_def (subst_instance u) (subst_instance u).
+
+Global Instance subst_instance_prod {A B} `(UnivSubst A) `(UnivSubst B)
+  : UnivSubst (A × B)
+  := fun u => on_pair (subst_instance u) (subst_instance u).
+
+Global Instance subst_instance_nat : UnivSubst nat
+  := fun _ n => n.
+
+
+
+Lemma subst_instance_instance_length u1 u2 :
+  #|subst_instance_instance u2 u1| = #|u1|.
 Proof.
-  intros cf Σ Γ B x u univs H.
-Admitted.
+  unfold subst_instance_instance.
+  now rewrite map_length.
+Qed.
+  
+Lemma subst_instance_level_two u1 u2 l :
+  subst_instance_level u1 (subst_instance_level u2 l)
+  = subst_instance_level (subst_instance_instance u1 u2) l.
+Proof.
+  destruct l; cbn; try reflexivity.
+  unfold subst_instance_instance.
+  rewrite <- (map_nth (subst_instance_level u1)); reflexivity.
+Qed.
+
+Lemma subst_instance_univ_two u1 u2 s :
+  subst_instance_univ u1 (subst_instance_univ u2 s)
+  = subst_instance_univ (subst_instance_instance u1 u2) s.
+Proof.
+  unfold subst_instance_univ. rewrite NEL.map_map.
+  apply NEL.map_ext. clear s.
+  intros [l []]; unfold subst_instance_level_expr;
+    now rewrite subst_instance_level_two.
+Qed.
+
+Lemma subst_instance_instance_two u1 u2 u :
+  subst_instance_instance u1 (subst_instance_instance u2 u)
+  = subst_instance_instance (subst_instance_instance u1 u2) u.
+Proof.
+  unfold subst_instance_instance. rewrite map_map.
+  apply map_ext, subst_instance_level_two.
+Qed.
 
 Lemma subst_instance_constr_two u1 u2 t :
-  subst_instance_constr u1 (subst_instance_constr u2 t) = subst_instance_constr (subst_instance_instance u1 u2) t.
+  subst_instance_constr u1 (subst_instance_constr u2 t)
+  = subst_instance_constr (subst_instance_instance u1 u2) t.
 Proof.
-Admitted.
+  induction t using term_forall_list_ind; cbn; f_equal;
+    auto using subst_instance_instance_two.
+  - rewrite map_map. now apply All_map_eq.
+  - apply subst_instance_univ_two.
+  - rewrite map_map. apply All_map_eq.
+    eapply All_impl; tea.
+    cbn. intros [? ?]; unfold on_snd; cbn; congruence.
+  - rewrite map_map. apply All_map_eq.
+    eapply All_impl; tea.
+    cbn. intros [? ? ?] [? ?]; cbn in *. unfold map_def; cbn; congruence.
+  - rewrite map_map. apply All_map_eq.
+    eapply All_impl; tea.
+    cbn. intros [? ? ?] [? ?]; cbn in *. unfold map_def; cbn; congruence.
+Qed.
 
-Lemma consistent_ext_trans:
-  forall (cf : checker_flags) (Σ : global_env × universes_decl) (u : universe_instance) U,
-    consistent_instance_ext Σ U u ->
-    forall (u0 : universe_instance) (univs : universes_decl),
-      consistent_instance_ext (Σ.1, univs) Σ.2 u0 ->
-      consistent_instance_ext (Σ.1, univs) U (subst_instance_instance u0 u).
+Lemma subst_instance_context_two u1 u2 Γ :
+  subst_instance_context u1 (subst_instance_context u2 Γ)
+  = subst_instance_context (subst_instance_instance u1 u2) Γ.
 Proof.
-  intros.
-Admitted.
+  induction Γ; try reflexivity.
+  simpl. rewrite IHΓ; f_equal.
+  destruct a as [? [] ?]; unfold map_decl; cbn;
+    now rewrite !subst_instance_constr_two.
+Qed.
 
-Hint Resolve consistent_ext_trans. 
-(* Hint Resolve wf_local_subst_instance.  *)
-
-Lemma subst_instance_univ_super:
-  forall (l : Level.t) (u : universe_instance),
-    subst_instance_univ u (Universe.super l) = Universe.super (subst_instance_level u l).
+Lemma subst_instance_cstr_two u1 u2 c :
+  subst_instance_cstr u1 (subst_instance_cstr u2 c)
+  = subst_instance_cstr (subst_instance_instance u1 u2) c.
 Proof.
-  intros l u.
-Admitted.
+  destruct c as [[? ?] ?]; unfold subst_instance_cstr; cbn.
+  now rewrite !subst_instance_level_two.
+Qed.
 
-
-Lemma subst_instance_univ_make :
-  forall (l : Level.t) (u : universe_instance),
-    subst_instance_univ u (Universe.make l) = Universe.make (subst_instance_level u l).
+Lemma In_subst_instance_cstrs u c ctrs :
+  CS.In c (subst_instance_cstrs u ctrs)
+  <-> exists c', c = subst_instance_cstr u c' /\ CS.In c' ctrs.
 Proof.
-  intros l u.
-Admitted.
+  unfold subst_instance_cstrs.
+  rewrite CS.fold_spec.
+  transitivity (CS.In c CS.empty \/
+                exists c', c = subst_instance_cstr u c'
+                      /\ In c' (CS.elements ctrs)).
+  - generalize (CS.elements ctrs), CS.empty.
+    induction l; cbn.
+    + firstorder.
+    + intros t. etransitivity. eapply IHl. split; intros [HH|HH].
+      * destruct a as [[l1 a] l2]. apply CS.add_spec in HH.
+        destruct HH as [HH|HH].
+        right; eexists. split; [|left; reflexivity]. assumption.
+        now left.
+      * destruct HH as [c' ?]. right; exists c'; intuition.
+      * left. destruct a as [[l1 a] l2]. apply CS.add_spec.
+        now right.
+      * destruct HH as [c' [HH1 [?|?]]]; subst.
+        left; destruct c' as [[l1 c'] l2];
+          apply CS.add_spec; now left.
+        right; exists c'; intuition.
+  - rewrite ConstraintSetFact.empty_iff.
+    transitivity (exists c', c = subst_instance_cstr u c'
+                        /\ In c' (CS.elements ctrs)).
+    intuition.
+    apply iff_ex; intro. apply and_iff_compat_l. symmetry.
+    etransitivity. eapply CS.elements_spec1.
+    etransitivity. eapply SetoidList.InA_alt.
+    split; intro; eauto.
+    now destruct H as [? [[] ?]].
+Qed.
 
-Lemma LevelIn_subst_instance:
-  forall (cf : checker_flags) (Σ : global_env × universes_decl) (l : Level.t),
-    LevelSet.In l (global_ext_levels Σ) ->
-    forall (u : universe_instance) (univs : universes_decl),
-      consistent_instance_ext (Σ.1, univs) Σ.2 u ->
-      LevelSet.In (subst_instance_level u l) (global_ext_levels (Σ.1, univs)).
+Lemma In_subst_instance_cstrs' u c ctrs :
+  CS.In c ctrs ->
+  CS.In (subst_instance_cstr u c) (subst_instance_cstrs u ctrs).
 Proof.
-  intros cf Σ l H u univs H0.
-Admitted.
+  intro H. apply In_subst_instance_cstrs. now eexists.
+Qed.
+
+Lemma subst_instance_cstrs_two u1 u2 ctrs :
+  CS.Equal
+    (subst_instance_cstrs u1 (subst_instance_cstrs u2 ctrs))
+    (subst_instance_cstrs (subst_instance_instance u1 u2) ctrs).
+Proof.
+  intro c; split; intro Hc; apply In_subst_instance_cstrs.
+  - apply In_subst_instance_cstrs in Hc; destruct Hc as [c' [eq Hc']].
+    apply In_subst_instance_cstrs in Hc'; destruct Hc' as [c'' [eq' Hc'']].
+    exists c''. subst; now rewrite subst_instance_cstr_two.
+  - apply In_subst_instance_cstrs in Hc; destruct Hc as [c' [eq Hc']].
+    exists (subst_instance_cstr u2 c'). split.
+    now rewrite subst_instance_cstr_two.
+    now apply In_subst_instance_cstrs'.
+Qed.
+
+
+Lemma consistent_instance_no_prop lvs φ uctx u :
+  consistent_instance lvs φ uctx u
+  -> forallb (fun x => negb (Level.is_prop x)) u.
+Proof.
+  unfold consistent_instance. destruct uctx as [ctx|ctx|ctx].
+  destruct u; [reflexivity|discriminate].
+  2: destruct ctx as [ctx ?].
+  all: destruct (AUContext.repr ctx); intro H; apply H.
+Qed.
+
+Hint Resolve consistent_instance_no_prop : univ_subst.
+
+Lemma consistent_instance_declared lvs φ uctx u :
+  consistent_instance lvs φ uctx u
+  -> forallb (fun l => LS.mem l lvs) u.
+Proof.
+  unfold consistent_instance. destruct uctx as [ctx|ctx|ctx].
+  destruct u; [reflexivity|discriminate].
+  2: destruct ctx as [ctx ?].
+  all: destruct (AUContext.repr ctx); intro H; apply H.
+Qed.
+
+Lemma monomorphic_level_notin_AUContext s φ :
+  ~ LS.In (Level.Level s) (AUContext.levels φ).
+Proof.
+  destruct φ as [φ1 φ2].
+  intro H. apply (proj1 (LevelSetProp.of_list_1 _ _)) in H. cbn in H.
+  apply SetoidList.InA_alt in H.
+  destruct H as [? [? H]]; subst. revert H.
+  unfold mapi; generalize 0.
+  induction φ1; cbn. trivial.
+  intros n [H|H]. discriminate. eauto.
+Qed.
+
+Global Instance satisfies_equal_sets v :
+  Morphisms.Proper (Morphisms.respectful CS.Equal iff) (satisfies v).
+Proof.
+  intros φ1 φ2 H; split; intros HH c Hc; now apply HH, H.
+Qed.
+
+Global Instance satisfies_subsets v :
+  Morphisms.Proper (Morphisms.respectful CS.Subset (flip impl))
+                   (satisfies v).
+Proof.
+  intros φ1 φ2 H H2 c Hc; now apply H2, H.
+Qed.
+
+Hint Resolve subst_instance_cstrs_two
+     satisfies_equal_sets satisfies_subsets : univ_subst.
+
+
+Lemma val0_subst_instance_level u l v
+      (Hu : forallb (negb ∘ Level.is_prop) u)
+  : val0 v (subst_instance_level u l) = val0 (subst_instance_valuation u v) l.
+Proof.
+  destruct l; aa; cbn.
+  rewrite Znat.Z2Nat.id; auto.
+  apply (forallb_nth' n Level.lSet) in Hu.
+    destruct Hu as [[?l [HH1 HH2]]|HH1]; rewrite HH1; cbn.
+    destruct l; try discriminate; cbn.
+    apply Zorder.Zle_0_nat.
+    reflexivity.
+Qed.
+
+Lemma satisfies0_subst_instance_ctr u v c
+      (Hu : forallb (negb ∘ Level.is_prop) u)
+  : satisfies0 v (subst_instance_cstr u c)
+    <-> satisfies0 (subst_instance_valuation u v) c.
+Proof.
+  destruct c as [[l1 []] l2]; unfold subst_instance_cstr; cbn;
+    split; intro H; constructor; inv H.
+  all: rewrite <- ?val0_subst_instance_level; tea.
+  all: rewrite ?val0_subst_instance_level; tea.
+Qed.
+
+Lemma satisfies_subst_instance_ctr u v ctrs
+      (Hu : forallb (negb ∘ Level.is_prop) u)
+  : satisfies v (subst_instance_cstrs u ctrs)
+    <-> satisfies (subst_instance_valuation u v) ctrs.
+Proof.
+  split; intros Hv c Hc.
+  - apply satisfies0_subst_instance_ctr; tas. apply Hv.
+    apply In_subst_instance_cstrs. exists c; now split.
+  - apply In_subst_instance_cstrs in Hc.
+    destruct Hc as [c' [? Hc']]; subst.
+    apply satisfies0_subst_instance_ctr; auto.
+Qed.
+
+(** global constraints are monomorphic *)
+
+Lemma not_var_global_levels Σ (hΣ : wf Σ) :
+  LS.For_all (negb ∘ Level.is_var) (global_levels Σ).
+Proof.
+  induction hΣ as [|Σ d hΣ IH HH univs Hu Hd].
+  - intros l Hl. apply LevelSet_pair_In in Hl.
+    destruct Hl as [Hl|Hl]; subst; reflexivity.
+  - subst univs. intros l Hl. simpl in Hl; apply LS.union_spec in Hl.
+    destruct Hl as [Hl|Hl]; auto. clear -Hu Hl.
+    destruct d as [? [? ? [φ|?|?]]|? [? ? ? ? [φ|?|?]]]; cbn in *;
+      unfold monomorphic_levels_decl in *; cbn in *;
+      try now apply LS.empty_spec in Hl.
+    all: destruct Hu as [_ [_ [Hu _]]];
+      apply LevelSetFact.for_all_2 in Hu; auto.
+    all: now intros x y [].
+Qed.
+
+Lemma not_var_global_ext_levels Σ φ (hΣ : wf_ext (Σ, Monomorphic_ctx φ)) :
+  LS.For_all (negb ∘ Level.is_var)
+                   (global_ext_levels (Σ, Monomorphic_ctx φ)).
+Proof.
+  destruct hΣ as [hΣ Hφ].
+  intros l Hl; apply LS.union_spec in Hl; destruct Hl as [Hl|Hl].
+  - destruct Hφ as [_ [_ [Hφ _]]]. apply LevelSetFact.for_all_2 in Hφ; auto.
+    now intros x y [].
+  - eapply not_var_global_levels; eassumption.
+Qed.
+
+Lemma levels_global_constraint Σ (hΣ : wf Σ) c :
+  CS.In c (global_constraints Σ)
+  -> LS.In c.1.1 (global_levels Σ)
+    /\ LS.In c.2 (global_levels Σ).
+Proof.
+  induction hΣ as [|Σ d hΣ IH HH univs Hu Hd].
+  - intro H; now apply CS.empty_spec in H.
+  - subst univs. intro Hc. simpl in *; apply CS.union_spec in Hc.
+    destruct Hc as [Hc|Hc]; auto. clear -Hu Hc.
+    + destruct d as [? [? ? [φ|?|?]]|? [? ? ? ? [φ|?|?]]]; cbn in *;
+        unfold monomorphic_levels_decl, monomorphic_constraints_decl in *; cbn in *;
+          try now apply CS.empty_spec in Hc.
+      all: destruct Hu as [_ [Hu [_ _]]].
+      all: destruct c as [[l1 c] l2]; exact (Hu _ Hc).
+    + split; apply LS.union_spec; now right.
+
+Qed.
+
+Lemma levels_global_ext_constraint Σ φ (hΣ : wf_ext (Σ, φ)) c :
+  CS.In c (global_ext_constraints (Σ, φ))
+  -> LS.In c.1.1 (global_ext_levels (Σ, φ))
+    /\ LS.In c.2 (global_ext_levels (Σ, φ)).
+Proof.
+  intro H. apply CS.union_spec in H; simpl in H.
+  destruct hΣ as [hΣ Hφ], H as [Hc|H]; simpl in *.
+  - destruct Hφ as [_ [Hφ _]]. unfold global_ext_levels. simpl.
+    destruct c as [[l1 c] l2]; exact  (Hφ _ Hc).
+  - apply levels_global_constraint in H; tas.
+    split; apply LS.union_spec; right; apply H.
+Qed.
+
+Definition is_monomorphic_cstr (c : univ_constraint)
+  := negb (Level.is_var c.1.1) && negb (Level.is_var c.2).
+
+Lemma monomorphic_global_constraint Σ (hΣ : wf Σ) c :
+  CS.In c (global_constraints Σ)
+  -> is_monomorphic_cstr c.
+Proof.
+  intros H. apply levels_global_constraint in H; tas.
+  apply andb_and. split; destruct H as [H1 H2].
+  now apply not_var_global_levels in H1.
+  now apply not_var_global_levels in H2.
+Qed.
+
+Lemma monomorphic_global_constraint_ext Σ φ 
+      (hΣ : wf_ext (Σ, Monomorphic_ctx φ)) c :
+  CS.In c (global_ext_constraints (Σ, Monomorphic_ctx φ))
+  -> is_monomorphic_cstr c.
+Proof.
+  intros H. apply levels_global_ext_constraint in H; tas.
+  apply andb_and. split; destruct H as [H1 H2].
+  now apply not_var_global_ext_levels in H1.
+  now apply not_var_global_ext_levels in H2.
+Qed.
+
+Hint Resolve monomorphic_global_constraint monomorphic_global_constraint_ext
+  : univ_subst.
+
+Lemma subst_instance_monom_cstr inst c :
+  is_monomorphic_cstr c
+  -> subst_instance_cstr inst c = c.
+Proof.
+  intro H; apply andb_and in H. destruct H.
+  destruct c as [[[] ?] []]; cbnr; discriminate.
+Qed.
+
+Lemma satisfies_union v φ1 φ2 :
+  satisfies v (CS.union φ1 φ2)
+  <-> (satisfies v φ1 /\ satisfies v φ2).
+Proof.
+  unfold satisfies. split.
+  - intros H; split; intros c Hc; apply H; now apply CS.union_spec.
+  - intros [H1 H2] c Hc; apply CS.union_spec in Hc; destruct Hc; auto.
+Qed.
+
+Lemma equal_subst_instance_cstrs_mono u cstrs :
+  CS.For_all is_monomorphic_cstr cstrs ->
+  CS.Equal (subst_instance_cstrs u cstrs) cstrs.
+Proof.
+  intros HH c. etransitivity.
+  eapply In_subst_instance_cstrs. split; intro H.
+  destruct H as [c' [eq Hc']]. subst; rewrite subst_instance_monom_cstr; aa.
+  exists c. rewrite subst_instance_monom_cstr; aa.
+Qed.
+
+Lemma subst_instance_cstrs_union u φ φ' :
+  CS.Equal (subst_instance_cstrs u (CS.union φ φ'))
+           (CS.union (subst_instance_cstrs u φ) (subst_instance_cstrs u φ')).
+Proof.
+  intro c; split; intro Hc.
+  - apply In_subst_instance_cstrs in Hc.
+    destruct Hc as [c' [eq Hc]]; subst.
+    apply* CS.union_spec in Hc.
+    destruct Hc; [left|right]; now apply In_subst_instance_cstrs'.
+  - apply In_subst_instance_cstrs.
+    apply CS.union_spec in Hc.
+    destruct Hc as [Hc|Hc]; apply In_subst_instance_cstrs in Hc;
+      destruct Hc as [c'[eq Hc]]; exists c'; aa; apply CS.union_spec;
+        [left|right]; aa.
+Qed.
+
+Hint Unfold CS.For_all : univ_subst.
+
+Definition sub_context_set (φ φ' : ContextSet.t)
+  := LS.Subset φ.1 φ'.1 /\ CS.Subset φ.2 φ'.2.
+
+Definition global_ext_context_set Σ : ContextSet.t
+  := (global_ext_levels Σ, global_ext_constraints Σ).
+
+Global Instance sub_context_set_trans : RelationClasses.Transitive sub_context_set.
+Proof.
+  split; (etransitivity; [eapply H | eapply H0]).
+Qed.
+
+
+Lemma consistent_ext_trans_polymorphic_case_aux {Σ φ1 φ2 φ' udecl inst inst'} :
+  wf_ext (Σ, Polymorphic_ctx (φ1, φ2)) ->
+  valid_constraints0 (global_ext_constraints (Σ, Polymorphic_ctx (φ1, φ2)))
+                     (subst_instance_cstrs inst udecl) ->
+  valid_constraints0 (global_ext_constraints (Σ, φ'))
+                     (subst_instance_cstrs inst' φ2) ->
+  forallb (fun x : Level.t => negb (Level.is_prop x)) inst' ->
+  valid_constraints0 (global_ext_constraints (Σ, φ'))
+                     (subst_instance_cstrs
+                        (subst_instance_instance inst' inst) udecl).
+Proof.
+  intros [HΣ Hφ] H3 H2 H2'.
+  intros v Hv. rewrite <- subst_instance_cstrs_two.
+  apply satisfies_subst_instance_ctr; tas. apply H3.
+  apply satisfies_union; simpl. split.
+  - apply satisfies_subst_instance_ctr; auto.
+  - apply satisfies_subst_instance_ctr; tas.
+    rewrite equal_subst_instance_cstrs_mono; aa.
+    apply satisfies_union in Hv; apply Hv.
+Qed.
+
+Lemma consistent_ext_trans_polymorphic_cases Σ φ φ' udecl inst inst' :
+  wf_ext (Σ, φ) ->
+  sub_context_set (monomorphic_udecl φ) (global_ext_context_set (Σ, φ')) ->
+  consistent_instance_ext (Σ, φ) (Polymorphic_ctx udecl) inst ->
+  consistent_instance_ext (Σ, φ') φ inst' ->
+  consistent_instance_ext (Σ, φ') (Polymorphic_ctx udecl)
+                          (subst_instance_instance inst' inst).
+Proof.
+  intros HΣφ Hφ [H [H0 [H1 H3]]] H2.
+  apply consistent_instance_no_prop in H2 as H2'.
+  repeat split.
+  3: now rewrite subst_instance_instance_length.
+  + clear -H H2'.
+    assert (HH: forall l, negb (Level.is_prop l) ->
+                     negb (Level.is_prop (subst_instance_level inst' l))). {
+      destruct l; cbnr; aa.
+      eapply (forallb_nth' n Level.lSet) in H2'.
+      destruct H2' as [[? [H2 ?]]|H2]; rewrite H2; auto. }
+    induction inst; cbnr. rewrite HH; cbn. apply IHinst.
+    all: apply andP in H; try apply H.
+  + rewrite forallb_map. apply forallb_forall.
+    intros l Hl. unfold global_ext_levels, compose in *; simpl in *.
+    eapply forallb_forall in H0; tea. clear -Hφ H0 H2 Hl.
+    apply LevelSet_mem_union in H0. destruct H0 as [H|H].
+    2: { destruct l; simpl; try (apply LevelSet_mem_union; right; assumption).
+         apply consistent_instance_declared in H2.
+         apply (forallb_nth' n Level.lSet) in H2.
+         destruct H2 as [[? [H2 ?]]|H2]; rewrite H2; tas.
+         apply LevelSet_mem_union; right.
+         apply global_levels_Set. }
+    *  destruct l; simpl.
+       -- apply LevelSet_mem_union; right; apply global_levels_Prop.
+       -- apply LevelSet_mem_union; right; apply global_levels_Set.
+       -- apply LS.mem_spec in H.
+          destruct φ as [φ|[φ1 φ2]|[[φ1 φ2] φ3]]; simpl in *.
+          apply Hφ in H. now apply LS.mem_spec.
+          all: now apply monomorphic_level_notin_AUContext in H.
+       -- apply consistent_instance_declared in H2.
+          apply (forallb_nth' n Level.lSet) in H2.
+          destruct H2 as [[? [H2 ?]]|H2]; rewrite H2; tas.
+          apply LevelSet_mem_union; right; apply global_levels_Set.
+  + unfold consistent_instance_ext, consistent_instance in H2.
+    unfold valid_constraints in *; destruct check_univs; [|trivial].
+    destruct φ as [φ|[φ1 φ2]|[[φ1 φ2] φ3]]; simpl in *.
+    * intros v Hv. rewrite <- subst_instance_cstrs_two.
+      apply satisfies_subst_instance_ctr; tas.
+      apply H3. apply satisfies_subst_instance_ctr; tas.
+      rewrite equal_subst_instance_cstrs_mono; aa.
+      apply satisfies_union; simpl; split.
+      -- intros c Hc. now apply Hv, Hφ.
+      -- apply satisfies_union in Hv; apply Hv.
+    * destruct H2 as [_ [_ [_ H2]]].
+      eapply consistent_ext_trans_polymorphic_case_aux; try eassumption.
+    * destruct H2 as [_ [_ [_ H2]]].
+      eapply (consistent_ext_trans_polymorphic_case_aux HΣφ); eassumption.
+Qed.
+
+Lemma consistent_ext_trans Σ φ φ' udecl inst inst' :
+  wf_ext (Σ, φ) ->
+  sub_context_set (monomorphic_udecl φ) (global_ext_context_set (Σ, φ')) ->
+  consistent_instance_ext (Σ, φ) udecl inst ->
+  consistent_instance_ext (Σ, φ') φ inst' ->
+  consistent_instance_ext (Σ, φ') udecl (subst_instance_instance inst' inst).
+Proof.
+  intros HΣφ Hφ H1 H2. destruct udecl as [?|udecl|[udecl ?]].
+  - (* udecl monomorphic *)
+    cbn; now rewrite subst_instance_instance_length.
+  - (* udecl polymorphic *)
+    eapply consistent_ext_trans_polymorphic_cases; eassumption.
+  - (* udecl cumulative *)
+    eapply consistent_ext_trans_polymorphic_cases; eassumption.
+Qed.
+
+Hint Resolve consistent_ext_trans : univ_subst.
+
+
+Lemma consistent_instance_valid_constraints Σ φ u univs :
+  wf_ext (Σ, φ) -> 
+  CS.Subset (monomorphic_constraints φ)
+                       (global_ext_constraints (Σ, univs)) ->
+  consistent_instance_ext (Σ, univs) φ u ->
+  valid_constraints (global_ext_constraints (Σ, univs))
+                    (subst_instance_cstrs u (global_ext_constraints (Σ, φ))).
+Proof.
+  intros HΣ Hsub HH.
+  apply consistent_instance_no_prop in HH as Hu.
+  unfold valid_constraints; case_eq check_univs; [intro Hcf|trivial].
+  intros v Hv. apply satisfies_subst_instance_ctr; tas.
+  apply satisfies_union; simpl; split.
+  - destruct φ as [φ|[φ1 φ2]|[[φ1 φ2] ?]].
+    + cbn. apply satisfies_subst_instance_ctr; tas.
+      rewrite equal_subst_instance_cstrs_mono; aa.
+      rewrite <- Hsub in Hv; assumption.
+      intros c Hc; eapply monomorphic_global_constraint_ext; tea.
+      apply CS.union_spec; now left.
+    + destruct HH as [_ [_ [_ H1]]].
+      unfold valid_constraints in H1; rewrite Hcf in H1.
+      apply satisfies_subst_instance_ctr; aa.
+    + destruct HH as [_ [_ [_ H1]]].
+      unfold valid_constraints in H1; rewrite Hcf in H1.
+      apply satisfies_subst_instance_ctr; aa.
+  - apply satisfies_subst_instance_ctr; tas.
+    rewrite equal_subst_instance_cstrs_mono; aa.
+    apply satisfies_union in Hv; apply Hv.
+Qed. 
+
+Hint Resolve consistent_instance_valid_constraints : univ_subst.
+
+Class SubstUnivPreserving {A} `{UnivSubst A} (R : constraints -> crelation A)
+  := Build_SubstUnivPreserving :
+       forall φ φ' (u : universe_instance),
+         forallb (fun x => negb (Level.is_prop x)) u ->
+         valid_constraints φ' (subst_instance_cstrs u φ) ->
+         subrelation (R φ)
+                     (precompose (R φ') (subst_instance u)).
+
+Lemma satisfies_subst_instance φ φ' u :
+  check_univs = true ->
+  forallb (fun x => negb (Level.is_prop x)) u ->
+  valid_constraints φ' (subst_instance_cstrs u φ) ->
+  forall v, satisfies v φ' ->
+       satisfies (subst_instance_valuation u v) φ.
+Proof.
+  intros Hcf Hu HH v Hv.
+  unfold valid_constraints in HH; rewrite Hcf in HH.
+  apply satisfies_subst_instance_ctr; aa.
+Qed.
+
+Global Instance leq_universe_subst_instance : SubstUnivPreserving leq_universe.
+Proof.
+  intros φ φ' u Hu HH t t' Htt'.
+  unfold leq_universe in *; case_eq check_univs;
+    [intro Hcf; rewrite Hcf in *|trivial].
+  intros v Hv; cbn.
+  rewrite !subst_instance_univ_val'; tas.
+  apply Htt'. clear t t' Htt'.
+  eapply satisfies_subst_instance; tea.
+Qed.
+
+Global Instance eq_universe_subst_instance : SubstUnivPreserving eq_universe.
+Proof.
+  intros φ φ' u Hu HH t t' Htt'.
+  unfold eq_universe in *; case_eq check_univs;
+    [intro Hcf; rewrite Hcf in *|trivial].
+  intros v Hv; cbn.
+  rewrite !subst_instance_univ_val'; tas.
+  apply Htt'. clear t t' Htt'.
+  eapply satisfies_subst_instance; tea.
+Qed.
+
+Lemma precompose_subst_instance_instance Rle u i i' :
+  precompose (R_universe_instance Rle) (subst_instance_instance u) i i'
+  <~> R_universe_instance (precompose Rle (subst_instance_univ u)) i i'.
+Proof.
+  unfold R_universe_instance, subst_instance_instance.
+  replace (map Universe.make (map (subst_instance_level u) i))
+    with (map (subst_instance_univ u) (map Universe.make i)).
+  replace (map Universe.make (map (subst_instance_level u) i'))
+    with (map (subst_instance_univ u) (map Universe.make i')).
+  split. apply All2_map_inv. apply All2_map.
+  all: rewrite !map_map; apply map_ext; reflexivity.
+Qed.
+
+Definition precompose_subst_instance_instance__1 Rle u i i'
+  := equiv _ _ (precompose_subst_instance_instance Rle u i i').
+
+Definition precompose_subst_instance_instance__2 Rle u i i'
+  := equiv_inv _ _ (precompose_subst_instance_instance Rle u i i').
+
+
+Global Instance eq_term_upto_univ_subst_instance
+         (Re Rle : constraints -> crelation universe)
+      {he: SubstUnivPreserving Re} {hle: SubstUnivPreserving Rle}
+  : SubstUnivPreserving (fun φ => eq_term_upto_univ (Re φ) (Rle φ)).
+Proof.
+  intros φ φ' u Hu HH t t'.
+  specialize (he _ _ _ Hu HH).
+  specialize (hle _ _ _ Hu HH).
+  clear Hu HH.
+  induction t in t', Rle, hle |- * using term_forall_list_ind;
+    inversion 1; subst; cbn; constructor;
+      eauto using precompose_subst_instance_instance__2, R_universe_instance_impl'.
+  all: apply All2_map; eapply All2_impl'; tea;
+    eapply All_impl; eauto; cbn; intros; aa.
+Qed.
+
+Lemma leq_term_subst_instance : SubstUnivPreserving leq_term.
+Proof. exact _. Qed.
+
+Lemma eq_term_subst_instance : SubstUnivPreserving eq_term.
+Proof. exact _. Qed.
+
+
+
+
+
+(** Now routine lemmas ... *)
+
+Lemma subst_instance_univ_super l u
+      (Hu : forallb (negb ∘ Level.is_prop) u)
+  : subst_instance_univ u (Universe.super l)
+    = Universe.super (subst_instance_level u l).
+Proof.
+  destruct l; cbnr. unfold subst_instance_level_expr; cbn.
+  destruct (le_lt_dec #|u| n) as [HH|HH].
+  + now rewrite nth_overflow.
+  + eapply (forallb_nth _ _ _ Level.lSet Hu) in HH.
+    destruct HH as [l [HH1 HH2]]. rewrite HH1.
+    destruct l; cbn; try reflexivity; discriminate.
+Qed.
+
+Lemma subst_instance_univ_make l u : 
+  subst_instance_univ u (Universe.make l)
+  = Universe.make (subst_instance_level u l).
+Proof.
+  reflexivity.
+Qed.
+
+
+Lemma LevelIn_subst_instance Σ l u univs :
+  LS.In l (global_ext_levels Σ) ->
+  LS.Subset (monomorphic_levels Σ.2) (global_ext_levels (Σ.1, univs)) ->
+  consistent_instance_ext (Σ.1, univs) Σ.2 u ->
+  LS.In (subst_instance_level u l) (global_ext_levels (Σ.1, univs)).
+Proof.
+  intros H H0 H'. destruct l; simpl.
+  - apply LS.union_spec; right; simpl.
+    apply LS.mem_spec, global_levels_Prop.
+  - apply LS.union_spec; right; simpl.
+    apply LS.mem_spec, global_levels_Set.
+  - apply LS.union_spec in H; destruct H as [H|H]; simpl in *.
+    + apply H0. destruct Σ as [? φ]; cbn in *; clear -H.
+      destruct φ as [?|?|[? ?]]; tas;
+        now apply monomorphic_level_notin_AUContext in H.
+    + apply LS.union_spec; now right.
+  - apply consistent_instance_declared in H'.
+    apply (forallb_nth' n Level.lSet) in H'.
+    destruct H' as [[? [eq ?]]|eq]; rewrite eq.
+    + now apply LS.mem_spec.
+    + apply LS.union_spec; right; simpl.
+      apply LS.mem_spec, global_levels_Set.
+Qed.
     
-Lemma product_subst_instance u s1 s2 :
-  subst_instance_univ u (Universe.sort_of_product s1 s2) = Universe.sort_of_product (subst_instance_univ u s1) (subst_instance_univ u s2).
-Admitted.
 
-Lemma iota_red_subst_instance :
-  forall (pars c : nat) (args : list term) (brs : list (nat × term)) u,
-    subst_instance_constr u (iota_red pars c args brs) =
-    iota_red pars c (map (subst_instance_constr u) args) (map (on_snd (subst_instance_constr u)) brs).
+Lemma is_prop_subst_instance_univ u l
+      (Hu : forallb (negb ∘ Level.is_prop) u)
+  : Universe.is_prop (subst_instance_univ u l) = Universe.is_prop l.
 Proof.
-  intros. unfold iota_red. rewrite !subst_instance_constr_mkApps. f_equal; auto using map_skipn.
+  assert (He : forall a, Universe.Expr.is_prop (subst_instance_level_expr u a)
+                    = Universe.Expr.is_prop a). {
+    intros [[] b]; cbn; try reflexivity.
+    destruct (le_lt_dec #|u| n) as [HH|HH].
+    + now rewrite nth_overflow.
+    + eapply (forallb_nth _ _ _ Level.lSet Hu) in HH.
+      destruct HH as [?l [HH1 HH2]]. rewrite HH1. now apply ssrbool.negbTE. }
+  induction l. apply He. cbn. f_equal. apply He. apply IHl.
+Qed.
+
+Lemma is_small_subst_instance_univ u l
+  : Universe.is_small l -> Universe.is_small (subst_instance_univ u l).
+Proof.
+  assert (He : forall a, Universe.Expr.is_small a ->
+             Universe.Expr.is_small (subst_instance_level_expr u a)). {
+    intros [[] []]; cbn; auto. }
+  induction l. apply He.
+  intro HH; cbn in HH; apply andP in HH; destruct HH as [H1 H2].
+  cbn. apply andb_and; split. now apply He.
+  now apply IHl.
+Qed.
+
+
+Lemma sup_subst_instance_univ u s1 s2 :
+  subst_instance_univ u (Universe.sup s1 s2)
+  = Universe.sup (subst_instance_univ u s1) (subst_instance_univ u s2).
+Proof.
+  unfold subst_instance_univ, Universe.sup.
+  apply NEL.map_app.
+Qed.
+
+Lemma product_subst_instance u s1 s2
+      (Hu : forallb (negb ∘ Level.is_prop) u)
+ : subst_instance_univ u (Universe.sort_of_product s1 s2)
+   = Universe.sort_of_product (subst_instance_univ u s1) (subst_instance_univ u s2).
+Proof.
+  unfold Universe.sort_of_product.
+  rewrite is_prop_subst_instance_univ; tas.
+  destruct (Universe.is_prop s2); cbn; try reflexivity.
+  apply sup_subst_instance_univ.
+Qed.
+
+
+Lemma iota_red_subst_instance pars c args brs u :
+  subst_instance_constr u (iota_red pars c args brs)
+  = iota_red pars c (subst_instance u args) (subst_instance u brs).
+Proof.
+  unfold iota_red. rewrite !subst_instance_constr_mkApps.
+  f_equal; simpl; eauto using map_skipn.
   rewrite nth_map; simpl; auto.
 Qed.
 
-Lemma fix_subst_subst_instance:
-  forall (u : universe_instance) (mfix : mfixpoint term),
-    fix_subst (map (map_def (subst_instance_constr u) (subst_instance_constr u)) mfix) =
-    map (subst_instance_constr u) (fix_subst mfix).
+Lemma fix_subst_subst_instance u mfix :
+  map (subst_instance_constr u) (fix_subst mfix)
+  = fix_subst (subst_instance u mfix).
 Proof.
-  intros u mfix.
-Admitted.
+  unfold fix_subst. rewrite map_length.
+  generalize #|mfix|. induction n. reflexivity.
+  simpl. rewrite IHn; reflexivity.
+Qed.
 
 
-Lemma cofix_subst_subst_instance:
-  forall (u : universe_instance) (mfix : mfixpoint term),
-    cofix_subst (map (map_def (subst_instance_constr u) (subst_instance_constr u)) mfix) =
-    map (subst_instance_constr u) (cofix_subst mfix).
+Lemma cofix_subst_subst_instance u mfix :
+  map (subst_instance_constr u) (cofix_subst mfix)
+  = cofix_subst (subst_instance u mfix).
 Proof.
-  intros u mfix.
-Admitted.
+  unfold cofix_subst. rewrite map_length.
+  generalize #|mfix|. induction n. reflexivity.
+  simpl. rewrite IHn; reflexivity.
+Qed.
 
 
-Lemma isConstruct_app_subst_instance:
-  forall (u : universe_instance) (t : term),
-    isConstruct_app (subst_instance_constr u t) = isConstruct_app t.
+Lemma isConstruct_app_subst_instance u t :
+  isConstruct_app (subst_instance_constr u t) = isConstruct_app t.
 Proof.
-  intros u t.
-Admitted.
+  unfold isConstruct_app.
+  assert (HH: (decompose_app (subst_instance_constr u t)).1
+              = subst_instance_constr u (decompose_app t).1). {
+    unfold decompose_app. generalize (@nil term) at 1. generalize (@nil term).
+    induction t; cbn; try reflexivity.
+    intros l l'. erewrite IHt1; reflexivity. }
+  rewrite HH. destruct (decompose_app t).1; reflexivity.
+Qed.
 
-Lemma red1_subst_instance {cf:checker_flags} (Σ : global_env_ext) Γ u s t :
-  wf Σ -> 
+Lemma fix_context_subst_instance u mfix :
+  subst_instance_context u (fix_context mfix)
+  = fix_context (subst_instance u mfix).
+Proof.
+  unfold subst_instance_context, map_context, fix_context.
+  rewrite map_rev. f_equal.
+  rewrite map_mapi, mapi_map. eapply mapi_ext.
+  intros n x. unfold map_decl, vass; cbn. f_equal.
+  symmetry; apply lift_subst_instance_constr.
+Qed.
+
+Lemma subst_instance_context_app u L1 L2 :
+  subst_instance_context u (L1,,,L2)
+  = subst_instance_context u L1 ,,, subst_instance_context u L2.
+Proof.
+  unfold subst_instance_context, map_context; now rewrite map_app.
+Qed.
+
+Lemma red1_subst_instance Σ Γ u s t :
   red1 Σ Γ s t ->
-  red1 Σ (subst_instance_context u Γ) (subst_instance_constr u s) (subst_instance_constr u t).
+  red1 Σ (subst_instance_context u Γ)
+       (subst_instance_constr u s) (subst_instance_constr u t).
 Proof.
+  intros X0. pose proof I as X.
   intros. induction X0 using red1_ind_all.
-  all: try now (cbn; econstructor; eauto).
+  all: try (cbn; econstructor; eauto; fail).
   - cbn. rewrite <- subst_subst_instance_constr. econstructor.
   - cbn. rewrite <- subst_subst_instance_constr. econstructor.
   - cbn. rewrite <- lift_subst_instance_constr. econstructor.
@@ -135,10 +796,9 @@ Proof.
       * destruct (isLambda (dbody d)) eqn:E2; inversion H.
         rewrite nth_error_map, E. cbn.
         destruct d. cbn in *. destruct dbody; cbn in *; try congruence.
-        repeat f_equal. rewrite <- subst_subst_instance_constr.
-        f_equal. eapply fix_subst_subst_instance.
-        rewrite fix_subst_subst_instance.
-        now rewrite subst_subst_instance_constr.
+        repeat f_equal.
+        all: rewrite <- subst_subst_instance_constr;
+          rewrite fix_subst_subst_instance; reflexivity.
       * inversion H.
     + unfold is_constructor in *.
       destruct (nth_error args narg) eqn:E; inversion H0; clear H0.
@@ -160,8 +820,8 @@ Proof.
     econstructor. fold subst_instance_constr.
     unfold unfold_cofix.
     rewrite nth_error_map. destruct nth_error; cbn.
-    rewrite cofix_subst_subst_instance.
-    rewrite subst_subst_instance_constr. all: now inversion E. 
+    rewrite <- subst_subst_instance_constr, cofix_subst_subst_instance.
+    all: now inversion E. 
   - cbn. rewrite subst_instance_constr_two. econstructor; eauto.
   - cbn. rewrite !subst_instance_constr_mkApps.
     econstructor. now rewrite nth_error_map, H.
@@ -178,8 +838,9 @@ Proof.
       eapply OnOne2_map; eapply OnOne2_impl; [ eassumption | ].
     intros. destruct X1. destruct p. inversion e. destruct x, y; cbn in *; subst.
     red. split; cbn; eauto.
-    rewrite fix_context_subst_instance.
-    unfold subst_instance_context, map_context in *. rewrite map_app in *. eassumption.
+    rewrite <- (fix_context_subst_instance u mfix0).
+    unfold subst_instance_context, map_context in *. rewrite map_app in *.
+    eassumption.
   - cbn; econstructor;
       eapply OnOne2_map; eapply OnOne2_impl; [ eassumption | ].
     intros. destruct X1. destruct p. inversion e. destruct x, y; cbn in *; subst.
@@ -188,181 +849,413 @@ Proof.
       eapply OnOne2_map; eapply OnOne2_impl; [ eassumption | ].
     intros. destruct X1. destruct p. inversion e. destruct x, y; cbn in *; subst.
     red. split; cbn; eauto.
-    rewrite fix_context_subst_instance.
-    unfold subst_instance_context, map_context in *. rewrite map_app in *. eassumption.
-    Grab Existential Variables. all:repeat econstructor.                                  
+    rewrite <- (fix_context_subst_instance u mfix0).
+    unfold subst_instance_context, map_context in *. rewrite map_app in *.
+    eassumption.
+    Grab Existential Variables. all:repeat econstructor.
 Qed.
 
-Lemma leq_term_subst_instance:
-  forall (cf : checker_flags) (Σ : global_env_ext) (u : universe_instance)
-    (univs : universes_decl),
-    consistent_instance_ext (Σ.1, univs) Σ.2 u ->
-    forall t u0 : term,
-      leq_term (global_ext_constraints Σ) t u0 ->
-      leq_term (global_ext_constraints (Σ.1, univs)) (subst_instance_constr u t)
-               (subst_instance_constr u u0).
-Proof.
-  intros cf Σ u univs H t u0 l.
-Admitted.
 
-Lemma cumul_subst_instance {cf:checker_flags} (Σ : global_env_ext) Γ u A B univs :
-  wf Σ ->
-  consistent_instance_ext (Σ.1,univs) (Σ.2) u ->
+
+Lemma cumul_subst_instance (Σ : global_env_ext) Γ u A B univs :
+  forallb (fun x => negb (Level.is_prop x)) u ->
+  valid_constraints (global_ext_constraints (Σ.1, univs))
+                    (subst_instance_cstrs u Σ) -> 
   Σ ;;; Γ |- A <= B ->
-  (Σ.1,univs) ;;; subst_instance_context u Γ |- (subst_instance_constr u A) <= (subst_instance_constr u B).
+  (Σ.1,univs) ;;; subst_instance_context u Γ
+                   |- subst_instance_constr u A <= subst_instance_constr u B.
 Proof.
-  intros. induction X0.
-  - econstructor. now eapply leq_term_subst_instance.    
-  - econstructor 2. eapply red1_subst_instance; eauto. eauto.
-  - econstructor 3. eauto. eapply red1_subst_instance; eauto.
+  intros Hu HH X0. induction X0.
+  - econstructor.
+    eapply leq_term_subst_instance; tea.
+  - econstructor 2. eapply red1_subst_instance; cbn; eauto. eauto.
+  - econstructor 3. eauto. eapply red1_subst_instance; cbn; eauto.
 Qed.
 
-Lemma subst_instance_context_app u L1 L2 :
-  subst_instance_context u (L1,,,L2) = subst_instance_context u L1 ,,, subst_instance_context u L2.
+Global Instance eq_decl_subst_instance : SubstUnivPreserving eq_decl.
 Proof.
-  unfold subst_instance_context, map_context; now rewrite map_app.
+  intros φ1 φ2 u Hu HH [? [?|] ?] [? [?|] ?] [H1 H2]; split; cbn in *; auto.
+  all: eapply eq_term_subst_instance; tea.
 Qed.
 
-Lemma typing_subst_instance `{cf : checker_flags} :
-  forall Σ : global_env_ext, wf Σ ->
-  forall Γ, wf_local Σ Γ ->
-  forall t T, Σ ;;; Γ |- t : T ->
-    forall u univs,
-      consistent_instance_ext (Σ.1,univs) (Σ.2) u ->
-      wf_local (Σ.1, univs) (subst_instance_context u Γ) ->
-      (Σ.1,univs) ;;; subst_instance_context u Γ |- subst_instance_constr u t : subst_instance_constr u T.
+Global Instance eq_context_subst_instance : SubstUnivPreserving eq_context.
 Proof.
-  apply (typing_ind_env (fun Σ Γ t T =>
-                           forall u univs,
-                             consistent_instance_ext (Σ.1,univs) (Σ.2) u ->
-                             wf_local (Σ.1, univs) (subst_instance_context u Γ) ->
-      (Σ.1,univs) ;;; _ |- PCUICUnivSubst.subst_instance_constr u t : PCUICUnivSubst.subst_instance_constr u T)); intros; cbn -[PCUICUnivSubst.subst_instance_constr] in *.
-  - cbn. rewrite <- lift_subst_instance_constr.
-    rewrite map_decl_type. econstructor.
-    eauto.
-    unfold subst_instance_context, map_context.
-    now rewrite nth_error_map, H.
-  - cbn -[Universe.make]. rewrite subst_instance_univ_super, subst_instance_univ_make.
-    econstructor. eauto. eapply LevelIn_subst_instance; eauto.
-  - cbn. 
+  intros φ φ' u Hu HH Γ Γ' X. eapply All2_map, All2_impl; tea.
+  eapply eq_decl_subst_instance; eassumption.
+Qed.
 
-    rewrite product_subst_instance. econstructor. eapply X1; eauto.
-    eapply X3; eauto. econstructor. eauto. cbn.
-    econstructor. cbn in X1. eapply X1 in X4; eauto.
-  - cbn. econstructor. eapply X1. eauto. eauto. eapply X3. eauto.
-    econstructor.  cbn in X1. eauto. cbn. eapply X1 in X4; eauto.
-  - cbn. econstructor; eauto. eapply X5. eauto.
-    econstructor.  cbn in X1. eauto. cbn. eapply X1 in X6; eauto.
-    cbn. eapply X3 in X6. eauto. eauto.
-  - cbn. unfold subst1. rewrite <- subst_subst_instance_constr. cbn. econstructor.
-    + cbn. eapply X1; eauto.
-    + eapply X3; eauto.
-  - cbn. rewrite subst_instance_constr_two. econstructor; eauto.
-  - cbn. erewrite <- (@ind_type_map (fun _ => subst_instance_constr u)).
-    erewrite <- (@ind_type_map (fun _ => subst_instance_constr u0)).
-    destruct idecl as [a b c d e] eqn:E. cbn.       
-    assert (b = (idecl.(ind_type))) as -> by now subst.
+Lemma subst_instance_destArity Γ A u :
+  destArity (subst_instance_context u Γ) (subst_instance_constr u A)
+  = match destArity Γ A with
+    | Some (ctx, s) => Some (subst_instance_context u ctx, subst_instance_univ u s)
+    | None => None
+    end.
+Proof.
+  induction A in Γ |- *; simpl; try reflexivity.
+  - change (subst_instance_context u Γ,, vass na (subst_instance_constr u A1))
+      with (subst_instance_context u (Γ ,, vass na A1)).
+    now rewrite IHA2.
+  - change (subst_instance_context u Γ ,,
+               vdef na (subst_instance_constr u A1) (subst_instance_constr u A2))
+      with (subst_instance_context u (Γ ,, vdef na A1 A2)).
+    now rewrite IHA3.
+Qed.
+
+
+(* todo move *)
+Lemma option_map_two {A B C} (f : A -> B) (g : B -> C) x
+  : option_map g (option_map f x) = option_map (g ∘ f) x.
+Proof.
+  destruct x; reflexivity.
+Qed.
+
+Lemma option_map_ext {A B} (f g : A -> B) (H : forall x, f x = g x)
+  : forall z, option_map f z = option_map g z.
+Proof.
+  intros []; cbn; congruence.
+Qed.
+
+
+Lemma subst_instance_instantiate_params_subst u0 params pars s ty :
+  option_map (on_pair (map (subst_instance_constr u0)) (subst_instance_constr u0))
+             (instantiate_params_subst params pars s ty)
+  = instantiate_params_subst (subst_instance_context u0 params)
+                             (map (subst_instance_constr u0) pars)
+                             (map (subst_instance_constr u0) s)
+                             (subst_instance_constr u0 ty).
+Proof.
+  induction params in pars, s, ty |- *; cbn.
+  - destruct pars; cbnr.
+  - destruct ?; cbnr; destruct ?; cbnr.
+    + rewrite IHparams; cbn. repeat f_equal.
+      symmetry; apply subst_subst_instance_constr.
+    + destruct ?; cbnr. now rewrite IHparams.
+Qed.
+
+Lemma subst_instance_instantiate_params u0 params pars ty :
+  option_map (subst_instance_constr u0)
+             (instantiate_params params pars ty)
+  = instantiate_params (subst_instance_context u0 params)
+                       (map (subst_instance_constr u0) pars)
+                       (subst_instance_constr u0 ty).
+Proof.
+  unfold instantiate_params.
+  change (@nil term) with (map (subst_instance_constr u0) []) at 2.
+  rewrite rev_subst_instance_context.
+  rewrite <- subst_instance_instantiate_params_subst.
+  destruct ?; cbnr. destruct p; cbn.
+  now rewrite subst_subst_instance_constr.
+Qed.
+
+Lemma subst_instance_inds u0 ind u bodies :
+  subst_instance u0 (inds ind u bodies)
+  = inds ind (subst_instance u0 u) bodies.
+Proof.
+  unfold inds.
+  induction #|bodies|; cbnr.
+  f_equal. apply IHn.
+Qed.
+
+
+Lemma subst_instance_decompose_prod_assum u Γ t :
+  subst_instance u (decompose_prod_assum Γ t)
+  = decompose_prod_assum (subst_instance_context u Γ) (subst_instance_constr u t).
+Proof.
+  induction t in Γ |- *; cbnr.
+  apply IHt2. apply IHt3.
+Qed.
+
+Lemma subst_instance_decompose_app_rec u Γ t
+  : subst_instance u (decompose_app_rec t Γ)
+    = decompose_app_rec (subst_instance u t) (subst_instance u Γ).
+Proof.
+  induction t in Γ |- *; cbnr.
+  now rewrite IHt1.
+Qed.
     
-    rewrite subst_instance_constr_two. econstructor.
-    2:{ rewrite E in *. clear E. cbn in *. eassumption. }
-    2:{ rewrite E in *. clear E. cbn in *.         
-        eapply consistent_ext_trans; eauto. }
-    eauto.
-  - cbn. admit.                  (* type of constructor *)
-  - cbn. rewrite subst_instance_constr_mkApps in *.
-    rewrite map_app. cbn. rewrite map_skipn. econstructor; eauto.
-    + admit.                          (* types_of_case *)
-    + admit.                          (* check_correct_arity *)
-    + eapply X4 in H3. rewrite subst_instance_constr_mkApps in H3. eassumption. eauto.
-    + eapply All2_map with (f := (on_snd (subst_instance_constr u0))) (g:= (on_snd (subst_instance_constr u0))). eapply All2_impl. eassumption. intros.
+Lemma subst_instance_to_extended_list u l
+  : map (subst_instance_constr u) (to_extended_list l)
+    = to_extended_list (subst_instance_context u l).
+Proof.
+  - unfold to_extended_list, to_extended_list_k.
+    change [] with (map (subst_instance_constr u) []) at 2.
+    generalize (@nil term), 0. induction l as [|[aa [ab|] ac] bb].
+    + reflexivity.
+    + intros l n; cbn. now rewrite IHbb.
+    + intros l n; cbn. now rewrite IHbb.
+Qed.
+
+Lemma subst_instance_build_branches_type u0 ind mdecl idecl pars u p :
+  map (option_map (on_snd (subst_instance_constr u0)))
+      (build_branches_type ind mdecl idecl pars u p)
+  = build_branches_type ind mdecl idecl (map (subst_instance_constr u0) pars)
+                        (subst_instance_instance u0 u) (subst_instance_constr u0 p).
+Proof.
+  rewrite !build_branches_type_. rewrite map_mapi.
+  eapply mapi_ext.
+  intros n [[id t] k]; cbn.
+  rewrite <- subst_instance_context_two.
+  rewrite <- subst_instance_constr_two.
+  rewrite <- subst_instance_inds.
+  rewrite subst_subst_instance_constr.
+  rewrite <- subst_instance_instantiate_params.
+  rewrite !option_map_two. apply option_map_ext.
+  intros x. rewrite <- (subst_instance_decompose_prod_assum u0 [] x).
+  destruct (decompose_prod_assum [] x). simpl.
+  unfold decompose_app; rewrite <- (subst_instance_decompose_app_rec u0 [] t0).
+  destruct (decompose_app_rec t0 []); cbn.
+  unfold subst_instance, subst_instance_list.
+  case_eq (chop (ind_npars mdecl) l); intros l0 l1 H. 
+  eapply chop_map in H; rewrite H; clear H.
+  unfold on_snd; cbn. f_equal.
+  rewrite subst_instance_constr_it_mkProd_or_LetIn. f_equal.
+  rewrite subst_instance_constr_mkApps; f_equal.
+  - rewrite subst_instance_context_length.
+    symmetry; apply lift_subst_instance_constr.
+  - rewrite map_app; f_equal; cbn.
+    rewrite subst_instance_constr_mkApps, map_app; cbn; repeat f_equal.
+    apply subst_instance_to_extended_list.
+Qed.
+
+
+Axiom fix_guard_subst_instance :
+  forall mfix u,
+    fix_guard mfix ->
+    fix_guard (map (map_def (subst_instance_constr u) (subst_instance_constr u))
+                   mfix).
+
+
+Lemma All_local_env_over_subst_instance Σ Γ (wfΓ : wf_local Σ Γ) :
+  All_local_env_over typing
+                     (fun Σ0 Γ0 (_ : wf_local Σ0 Γ0) t T (_ : Σ0;;; Γ0 |- t : T) =>
+       forall u univs, wf_ext Σ0 ->
+                  sub_context_set (monomorphic_udecl Σ0.2)
+                                  (global_ext_context_set (Σ0.1, univs)) ->
+                  consistent_instance_ext (Σ0.1, univs) Σ0.2 u ->
+                  (Σ0.1, univs) ;;; subst_instance_context u Γ0
+                  |- subst_instance_constr u t : subst_instance_constr u T)
+                     Σ Γ wfΓ ->
+  forall u univs,
+    wf_ext Σ ->
+    sub_context_set (monomorphic_udecl Σ.2)
+                    (global_ext_context_set (Σ.1, univs)) ->
+    consistent_instance_ext (Σ.1, univs) Σ.2 u ->
+    wf_local (Σ.1, univs) (subst_instance_context u Γ).
+Proof.
+  induction 1; simpl; constructor; cbn in *; auto.
+  all: destruct tu; eexists; cbn in *; eauto.
+Qed.
+
+Hint Resolve All_local_env_over_subst_instance : univ_subst.
+
+Lemma typing_subst_instance :
+  env_prop (fun Σ Γ t T => forall u univs,
+                wf_ext Σ ->
+                sub_context_set (monomorphic_udecl Σ.2)
+                                (global_ext_context_set (Σ.1, univs)) ->
+                consistent_instance_ext (Σ.1, univs) Σ.2 u ->
+                (Σ.1,univs) ;;; subst_instance_context u Γ
+                |- subst_instance_constr u t : subst_instance_constr u T).
+Proof.
+  apply typing_ind_env; intros Σ wfΣ Γ wfΓ; cbn  -[Universe.make] in *.
+  - intros n decl eq X u univs wfΣ' H Hsub. rewrite <- lift_subst_instance_constr.
+    rewrite map_decl_type. econstructor; aa.
+    unfold subst_instance_context, map_context.
+    now rewrite nth_error_map, eq.
+  - intros l X Hl u univs wfΣ' HSub H.
+    rewrite subst_instance_univ_super, subst_instance_univ_make.
+    econstructor. aa. destruct HSub. eapply LevelIn_subst_instance; eauto.
+    eapply consistent_instance_no_prop; eassumption.
+  - intros n t0 b s1 s2 X X0 X1 X2 X3 u univs wfΣ' HSub H.
+    rewrite product_subst_instance; aa. econstructor.
+    eapply X1; eauto.
+    eapply X3; eauto.
+  - intros n t0 b s1 bty X X0 X1 X2 X3 u univs wfΣ' HSub H.
+    econstructor. eapply X1; aa. eapply X3; aa.
+  - intros n b b_ty b' s1 b'_ty X X0 X1 X2 X3 X4 X5 u univs wfΣ' HSub H.
+    econstructor; eauto. eapply X5; aa.
+  - intros t0 na A B u X X0 X1 X2 X3 u0 univs wfΣ' HSub H.
+    rewrite <- subst_subst_instance_constr. cbn. econstructor.
+    + eapply X1; eauto.
+    + eapply X3; eauto.
+  - intros. rewrite subst_instance_constr_two. econstructor; [aa|aa|].
+    clear X X0; cbn in *.
+    eapply consistent_ext_trans; eauto.
+  - intros. rewrite subst_instance_constr_two. econstructor; [aa|aa|].
+    clear X X0; cbn in *.
+    eapply consistent_ext_trans; eauto.
+  - intros. eapply meta_conv. econstructor; aa. clear.
+    unfold type_of_constructor; cbn.
+    rewrite <- subst_subst_instance_constr. f_equal.
+    + unfold inds. induction #|ind_bodies mdecl|. reflexivity.
+      cbn. now rewrite IHn.
+    + symmetry; apply subst_instance_constr_two.
+  - intros ind u npar p c brs args mdecl idecl isdecl X X0 H pty X1 indctx pctx ps
+           btys H0 X2 H1 X3 X4 X5 X6 u0 univs wfΣ' HSub H2.
+    rewrite subst_instance_constr_mkApps in *.
+    rewrite map_app. cbn. rewrite map_skipn.
+    eapply type_Case with (u1:=subst_instance_instance u0 u)
+                          (indctx0:=subst_instance_context u0 indctx)
+                          (ps0 :=subst_instance_univ u0 ps)
+                          (pctx0:=subst_instance_context u0 pctx)
+                          (btys0:=map (on_snd (subst_instance_constr u0)) btys);
+      eauto.
+
+    + clear -H0 H2. rewrite firstn_map.
+      apply* types_of_case_spec in H0. destruct H0 as [s' [E1 [E2 E3]]].
+      eexists. repeat split.
+      2: now rewrite (subst_instance_destArity []), E2.
+      * rewrite <- subst_instance_constr_two, <- subst_instance_context_two.
+        set (param' := subst_instance_context u (ind_params mdecl)) in *.
+        set (type' := subst_instance_constr u (ind_type idecl)) in *.
+        rewrite <- subst_instance_instantiate_params.
+        destruct (instantiate_params param' (firstn npar args) type');
+          [|discriminate].
+        cbn in *. apply some_inj in E1.
+        rewrite (subst_instance_destArity []), E1; reflexivity.
+      * rewrite <- subst_instance_build_branches_type.
+        now rewrite map_option_out_map_option_map, E3.
+    + clear -X2 X HSub wfΣ' H2. destruct HSub as [_ HSub]; cbn in *.
+      eapply consistent_instance_valid_constraints in H2 as H2'; aa; simpl in *.
+      eapply eq_context_subst_instance in X2; aa.
+      refine (transport (fun c => eq_context _ c _) _ X2). clear.
+      cbn. f_equal. unfold map_decl; cbn. f_equal.
+      rewrite subst_instance_constr_mkApps. f_equal.
+      rewrite !map_app. f_equal.
+      * rewrite firstn_map, !map_map. eapply map_ext.
+        rewrite subst_instance_context_length.
+        intro; symmetry; apply lift_subst_instance_constr.
+      * apply subst_instance_to_extended_list.
+    + clear -H1 H2. induction H1.
+      -- constructor 1. unfold universe_family in *.
+         rewrite is_prop_subst_instance_univ; aa.
+         destruct (Universe.is_prop ps); aa.
+         case_eq (Universe.is_small ps); intro HH; rewrite HH in H.
+         ++ apply (is_small_subst_instance_univ u0) in HH.
+            now rewrite HH.
+         ++ admit.  (* FIXME: InType not stable under substituion *)
+      -- constructor 2; auto.
+    + apply X5 in H2; tea.
+      rewrite subst_instance_constr_mkApps in H2; eassumption.
+    + eapply All2_map with (f := (on_snd (subst_instance_constr u0)))
+                           (g:= (on_snd (subst_instance_constr u0))).
+      eapply All2_impl. eassumption. intros.
       destruct X7. destruct p0. split. cbn. eauto. cbn.
       destruct x, y; cbn in *; subst.
-      eapply t. eauto. eauto.
-  - cbn. unfold subst1. rewrite <- subst_subst_instance_constr. cbn.
+      eapply t; assumption.
+  - intros p c u mdecl idecl pdecl isdecl args X X0 X1 X2 H u0 univs wfΣ' HSub H0.
+    rewrite <- subst_subst_instance_constr. cbn.
     rewrite !subst_instance_constr_two.
     rewrite map_rev. econstructor; eauto. 2:now rewrite map_length.
-    eapply X2 in H0. rewrite subst_instance_constr_mkApps in H0.
-    eassumption. eauto.
-  - cbn.
+    eapply X2 in H0; tas. rewrite subst_instance_constr_mkApps in H0.
+    eassumption.
+  - intros mfix n decl H H0 X X0 u univs wfΣ' HSub H1.
+    erewrite map_dtype. econstructor.
+    + now apply fix_guard_subst_instance.
+    + rewrite nth_error_map, H. reflexivity.
+    + rewrite <- (fix_context_subst_instance u mfix).
+      refine (subst_instance_context_app u Γ (fix_context mfix) # _).
+      destruct mfix; [cbn in; rewrite nth_error_nil in H; discriminate|].
+      inv X0. eapply typing_wf_local. eapply X1; eassumption.
+    + eapply All_map, All_impl; tea.
+      intros x [[X1 X2] X3]. split.
+      * specialize (X3 u univs wfΣ' HSub H1). erewrite map_dbody in X3.
+        rewrite <- lift_subst_instance_constr in X3.
+        rewrite fix_context_length, map_length in *.
+        erewrite map_dtype with (d := x) in X3.
+        unfold subst_instance_context, map_context in *.
+        rewrite map_app in *.
+        rewrite <- (fix_context_subst_instance u mfix).
+        eapply X3.
+      * destruct x as [? ? []]; cbn in *; tea.
+  - intros mfix n decl H X X0 H0 u univs wfΣ' HSub H1.
+    erewrite map_dtype. econstructor; tas.
+    + rewrite nth_error_map, H. reflexivity.
+    + rewrite <- (fix_context_subst_instance u mfix).
+      refine (subst_instance_context_app u Γ (fix_context mfix) # _).
+      destruct mfix; [cbn in; rewrite nth_error_nil in H; discriminate|].
+      inv X0. eapply typing_wf_local. eapply X1; eassumption.
+    + eapply All_map, All_impl; tea.
+      intros x [X1 X3].
+      * specialize (X3 u univs wfΣ' HSub H1). erewrite map_dbody in X3.
+        rewrite <- lift_subst_instance_constr in X3.
+        rewrite fix_context_length, map_length in *.
+        erewrite map_dtype with (d := x) in X3.
+        unfold subst_instance_context, map_context in *.
+        rewrite map_app in *.
+        rewrite <- (fix_context_subst_instance u mfix).
+        eapply X3.
 
-    assert (Hw :  wf_local (Σ.1, univs) (subst_instance_context u (Γ ,,, types))).
-    { (* rewrite subst_instance_context_app. *)
-      apply All_local_env_app in X as [X Hfixc].
-      
-      revert Hfixc. clear - H1 X1.
-      induction 1.
-      - eauto.
-      - cbn. econstructor; eauto. cbn in *.
-        destruct t0 as (? & ? & ?). eexists.
-        eapply t1 in H1. eapply H1. eauto.
-      - cbn. econstructor; eauto. cbn in *.
-        destruct t0 as (? & ? & ?). eexists.
-        eapply t2 in H1. eapply H1. eauto.
-        cbn. eapply t1 in H1. eapply H1. eauto.
-    } 
-
-    erewrite map_dtype. econstructor. admit. (* fix_guard *)
-    rewrite nth_error_map, H. cbn. reflexivity. destruct mfix. destruct n; inv H. eapply typing_wf_local.
-
-    inv X0. destruct X2. eapply t in H1.
-    
-    unfold subst_instance_context, map_context, app_context in *.
-    rewrite map_app in H1. subst types.
-    rewrite fix_context_subst_instance. eassumption.
-    
-    eauto.
-    
-    eapply All_map. eapply All_impl. eassumption.
-    intros. cbn in *. destruct X2. destruct p. split.
-    + specialize (t u univs).  erewrite map_dbody in t.
-      rewrite <- lift_subst_instance_constr in *. subst. rewrite fix_context_length, map_length in *.
-      erewrite map_dtype with (d := x) in t.
-      unfold subst_instance_context, map_context in *.
-      rewrite map_app in *. subst types.
-
-      rewrite fix_context_subst_instance.
-      eapply t. eauto. eauto.
-    + cbn. destruct x. cbn in *. destruct dbody; cbn in *; congruence.
-  - cbn.
-    
-    assert (Hw :  wf_local (Σ.1, univs) (subst_instance_context u (Γ ,,, types))).
-    { (* rewrite subst_instance_context_app. *)
-      apply All_local_env_app in X as [X Hfixc].
-      
-      revert Hfixc. clear - H1 X1.
-      induction 1.
-      - eauto.
-      - cbn. econstructor; eauto. cbn in *.
-        destruct t0 as (? & ? & ?). eexists.
-        eapply t1 in H1. eapply H1. eauto.
-      - cbn. econstructor; eauto. cbn in *.
-        destruct t0 as (? & ? & ?). eexists.
-        eapply t2 in H1. eapply H1. eauto.
-        cbn. eapply t1 in H1. eapply H1. eauto.
-    } 
-
-    erewrite map_dtype. econstructor. admit. (* fix_guard *)
-    rewrite nth_error_map, H. cbn. reflexivity. destruct mfix. destruct n; inv H. eapply typing_wf_local.
-
-    inv X0. destruct X2. eapply t0 in H1.
-    
-    unfold subst_instance_context, map_context, app_context in *.
-    rewrite map_app in H1. subst types.
-    rewrite fix_context_subst_instance. eassumption. eauto.
-    
-    eapply All_map. eapply All_impl. eassumption.
-    intros. cbn in *. destruct X2. unfold compose.
-    cbn. specialize (t0 u univs).  erewrite map_dbody in t0.
-    rewrite <- lift_subst_instance_constr in *. subst. rewrite fix_context_length, map_length in *.
-    erewrite map_dtype with (d := x) in t.
-    unfold subst_instance_context, map_context in *.
-    rewrite map_app in *. subst types.
-
-    rewrite fix_context_subst_instance.
-    eapply t0. eauto. eauto.
-  - econstructor. eapply X1. eauto. eauto.
-    + destruct X2.
-      * destruct i as (? & ?). left. eapply isWfArity_subst_instance; eauto.
-      * destruct s as (? & ? & ?). right. eexists. eapply t1. eauto. eauto.
+  - intros t0 A B X X0 X1 X2 X3 u univs wfΣ' HSub H.
+    econstructor. eapply X1; aa.
+    + destruct X2; [left|right].
+      * clear -i H wfΣ' HSub. destruct i as [[ctx [s [H1 H2]]] HH]; cbn in HH.
+        exists (subst_instance_context u ctx), (subst_instance_univ u s). split.
+        now rewrite (subst_instance_destArity []), H1.
+        rewrite <- subst_instance_context_app. unfold app_context in *.
+        revert H2 HH. generalize (ctx ++ Γ).
+        induction 1; simpl; constructor; auto; cbn in *.
+        eexists. eapply p; tas.
+        eexists. eapply p0; tas.
+        eapply p; tas.
+      * aa.
     + eapply cumul_subst_instance; eauto.
 Admitted.
+
+
+Lemma typing_subst_instance' Σ φ Γ t T u univs :
+  wf_ext (Σ, univs) ->
+  (Σ, univs) ;;; Γ |- t : T ->
+  sub_context_set (monomorphic_udecl univs) (global_ext_context_set (Σ, φ)) ->
+  consistent_instance_ext (Σ, φ) univs u ->
+  (Σ, φ) ;;; subst_instance_context u Γ
+            |- subst_instance_constr u t : subst_instance_constr u T.
+Proof.
+  intros X X0 X1.
+  eapply (typing_subst_instance (Σ, univs)); tas. apply X.
+  eapply typing_wf_local; eassumption.
+Qed.
+
+
+Definition global_context_set Σ : ContextSet.t
+  := (global_levels Σ, global_constraints Σ).
+
+Lemma global_context_set_sub_ext Σ φ :
+  sub_context_set (global_context_set Σ) (global_ext_context_set (Σ, φ)).
+Proof.
+  split. cbn. apply LevelSetProp.union_subset_2.
+  apply ConstraintSetProp.union_subset_2.
+Qed.
+
+
+Lemma weaken_lookup_on_global_env'' Σ c decl :
+  wf Σ ->
+  lookup_env Σ c = Some decl ->
+  sub_context_set (monomorphic_udecl (universes_decl_of_decl decl))
+                  (global_context_set Σ).
+Proof.
+  intros X1 X2; pose proof (weaken_lookup_on_global_env' _ _ _ X1 X2) as XX.
+  set (φ := universes_decl_of_decl decl) in *; clearbody φ. clear -XX.
+  destruct φ as [φ|φ|φ].
+  split; apply XX.
+  all: split;
+    [apply LevelSetProp.subset_empty|apply ConstraintSetProp.subset_empty].
+Qed.
+
+
+Lemma typing_subst_instance'' Σ φ Γ t T u univs :
+  wf_ext (Σ, univs) ->
+  (Σ, univs) ;;; Γ |- t : T ->
+  sub_context_set (monomorphic_udecl univs) (global_context_set Σ) ->
+  consistent_instance_ext (Σ, φ) univs u ->
+  (Σ, φ) ;;; subst_instance_context u Γ
+            |- subst_instance_constr u t : subst_instance_constr u T.
+Proof.
+  intros X X0 X1.
+  eapply (typing_subst_instance (Σ, univs)); tas. apply X.
+  eapply typing_wf_local; eassumption.
+  etransitivity; tea. apply global_context_set_sub_ext.
+Qed.
+
+
+End CheckerFlags.
