pcuic/theories/PCUICSafeLemmata.v
@@ -326,7 +326,7 @@ Section Lemmata.
   Proof.
     intros ind mdecl idecl npar args u p p' pty indctx pctx ps btys htc e.
     unfold types_of_case in *.
-    case_eq (instantiate_params (ind_params mdecl) (firstn npar args) (ind_type idecl)) ;
+    case_eq (instantiate_params (subst_instance_context u (ind_params mdecl)) (firstn npar args) (subst_instance_constr u (ind_type idecl))) ;
       try solve [ intro bot ; rewrite bot in htc ; discriminate htc ].
     intros ity eity. rewrite eity in htc.
     case_eq (destArity [] ity) ;
@@ -403,6 +403,7 @@ Section Lemmata.
       + cbn. eexists. eassumption.
       + cbn. eexists. eassumption.
   Qed.
+
 
   Lemma type_rename :
     forall Σ Γ u v A,
@@ -495,19 +496,19 @@ Section Lemmata.
         eapply eq_term_upto_univ_subst ; now auto.
     - intros cst u decl ? ? hdecl hcons v e.
       dependent destruction e.
-      apply All2_eq in a. apply map_inj in a ; revgoals.
+      apply All2_eq in r. apply map_inj in r ; revgoals.
       { intros x y h. inversion h. reflexivity. }
       subst.
       constructor ; auto.
     - intros ind u mdecl idecl isdecl ? ? hcons v e.
       dependent destruction e.
-      apply All2_eq in a. apply map_inj in a ; revgoals.
+      apply All2_eq in r. apply map_inj in r ; revgoals.
       { intros x y h. inversion h. reflexivity. }
       subst.
       econstructor ; eauto.
     - intros ind i u mdecl idecl cdecl isdecl ? ? ? v e.
       dependent destruction e.
-      apply All2_eq in a. apply map_inj in a ; revgoals.
+      apply All2_eq in r. apply map_inj in r ; revgoals.
       { intros x y h. inversion h. reflexivity. }
       subst.
       econstructor ; eauto.
@@ -1128,8 +1129,6 @@ Section Lemmata.
       Reflexive Rle ->
       Transitive Re ->
       Transitive Rle ->
-      SubstUnivPreserving Re ->
-      SubstUnivPreserving Rle ->
       (forall u u' : universe, Re u u' -> Rle u u') ->
       eq_term_upto_univ Re Rle u u' ->
       cored Σ Γ v u ->
@@ -1137,7 +1136,7 @@ Section Lemmata.
         cored Σ Γ v' u' /\
         ∥ eq_term_upto_univ Re Rle v v' ∥.
   Proof.
-    intros Re Rle Γ u v u' he hle tRe tRle hRe hRle hR e h.
+    intros Re Rle Γ u v u' he hle tRe tRle hR e h.
     induction h.
     - eapply red1_eq_term_upto_univ_l in X ; try exact e ; eauto.
       destruct X as [v' [r e']].
@@ -1993,7 +1992,7 @@ Proof.
   intros Σ Γ ind u p args mdecl idecl isdecl pars pty Hp indctx pctx ps btys e
          Hc.
   unfold types_of_case in e.
-  case_eq (instantiate_params (ind_params mdecl) pars (ind_type idecl));
+  case_eq (instantiate_params (subst_instance_context u (ind_params mdecl)) pars (subst_instance_constr u (ind_type idecl)));
     [|intro HH; rewrite HH in e; discriminate e].
   intros params' He; rewrite He in e.
   case_eq (destArity [] params');
